uncommenting LL and LVARS

examples/layeredeffects/LL.fst
@@ -83,251 +83,251 @@ layered_effect {
   if_then_else = eif_then_else
 }
 
-// inline_for_extraction
-// let lift_pure_exn (a:Type) (wp:pure_wp a{forall p q. (forall x. p x ==> q x) ==> (wp p ==> wp q)}) (f:unit -> PURE a wp)
-// : erepr a (fun p -> wp (fun x -> p (Some x)))
-// = fun _ -> Some (f ())
+inline_for_extraction
+let lift_pure_exn (a:Type) (wp:pure_wp a{forall p q. (forall x. p x ==> q x) ==> (wp p ==> wp q)}) (f:unit -> PURE a wp)
+: erepr a (fun p -> wp (fun x -> p (Some x)))
+= fun _ -> Some (f ())
 
-// sub_effect PURE ~> EXN = lift_pure_exn
+sub_effect PURE ~> EXN = lift_pure_exn
 
-// effect Exn (a:Type) (pre:Type0) (post:option a -> Type0) =
-//   EXN a (fun p -> pre /\ (forall r. post r ==> p r))
-
-
-
-// type pre_t = nat -> Type0
-// type post_t (a:Type) = option (a & nat) -> Type0
-// type wp_t0 (a:Type) = post_t a -> pre_t
-
-// unfold
-// let monotonic_wp (#a:Type) (wp:wp_t0 a) : Type0 =
-//   forall p q.
-//     (forall r. p r ==> q r) ==>
-//     (forall n. wp p n ==> wp q n)
-
-// type wp_t (a:Type) =
-//   wp:wp_t0 a{monotonic_wp wp}
-
-// type repr (a:Type) (wp:wp_t a) =
-//   n:nat -> EXN (a & nat) (fun p -> wp p n)
-
-// inline_for_extraction
-// let return (a:Type) (x:a)
-// : repr a (fun p n -> p (Some (x, n)))
-// = fun n -> (x, n)
-
-// unfold
-// let post_a (a:Type) (b:Type) (wp_g:a -> wp_t b) (p:post_t b) : post_t a =
-//   fun r ->
-//   match r with
-//   | None -> p None
-//   | Some r -> Prims.auto_squash (wp_g (Mktuple2?._1 r) p (Mktuple2?._2 r))
-
-// let lemma_monotonic2 (#a:Type) (#b:Type) (wp_f:wp_t a) (wp_g:a -> wp_t b) (p:post_t b) (q:post_t b) (n:nat)
-// : Lemma
-//   (requires forall (r:option (a & nat)). post_a a b wp_g p r ==> post_a a b wp_g q r)
-//   (ensures wp_f (post_a a b wp_g p) n ==> wp_f (post_a a b wp_g q) n)
-// = let aux (p q:post_t a)
-//     : Lemma ((forall r. p r ==> q r) ==> (forall n. wp_f p n ==> wp_f q n))
-//     = () in
-//   aux (post_a a b wp_g p) (post_a a b wp_g q)
-
-// unfold
-// let bind_wp0 (a:Type) (b:Type) (wp_f:wp_t a) (wp_g:a -> wp_t b) : post_t b -> pre_t =
-//   fun p n -> wp_f (post_a a b wp_g p) n
-
-// open FStar.Tactics
-
-// unfold
-// let bind_wp (a:Type) (b:Type) (wp_f:wp_t a) (wp_g:a -> wp_t b) : wp_t b
-// = assert (monotonic_wp (bind_wp0 a b wp_f wp_g)) by
-//     (norm [delta_only [`%monotonic_wp]];
-//      let p_binder = forall_intro () in
-//      let q_binder = forall_intro () in
-//      ignore (implies_intro ());
-//      ignore (forall_intro ());
-//      norm [delta_only [`%bind_wp0]];
-//      let wp_f_binder, wp_g_binder =
-//        match (cur_binders ()) with
-//        | _::_::wp_f::wp_g::_ -> wp_f, wp_g
-//        | _ -> fail "" in
-//      apply_lemma (`(lemma_monotonic2 (`#(binder_to_term wp_f_binder)) (`#(binder_to_term wp_g_binder)) (`#(binder_to_term p_binder)) (`#(binder_to_term q_binder))));
-//      norm [delta_only [`%post_a]];
-//      ignore (forall_intro ()));
-//   bind_wp0 a b wp_f wp_g
-
-// inline_for_extraction
-// let bind (a:Type) (b:Type)
-//   (wp_f:wp_t a) (wp_g:a -> wp_t b)
-//   (f:repr a wp_f) (g:(x:a -> repr b (wp_g x)))
-// : repr b (bind_wp a b wp_f wp_g)
-// = fun n ->
-//   let (x, n) = f n in
-//   g x n
-
-// inline_for_extraction
-// let subcomp (a:Type)
-//   (wp_f:wp_t a) (wp_g:wp_t a)
-//   (f:repr a wp_f)
-// : Pure (repr a wp_g)
-//   (requires forall p n. wp_g p n ==> wp_f p n)
-//   (ensures fun _ -> True)
-// = f
-
-// inline_for_extraction
-// let if_then_else (a:Type)
-//   (wp_f:wp_t a) (wp_g:wp_t a)
-//   (f:repr a wp_f) (g:repr a wp_g)
-//   (p:Type0)
-// : Type
-// = repr a
-//   (fun post n ->
-//     (p ==> wp_f post n) /\
-//     ((~ p) ==> wp_g post n))
-
-// reifiable reflectable
-// layered_effect {
-//   STEXN : a:Type -> wp:wp_t a -> Effect
-//   with
-//   repr = repr;
-//   return = return;
-//   bind = bind;
-//   subcomp = subcomp;
-//   if_then_else = if_then_else
-// }
-
-// inline_for_extraction
-// let lift_pure_stexn (a:Type) (wp:pure_wp a{forall p q. (forall x. p x ==> q x) ==> (wp p ==> wp q)}) (f:unit -> PURE a wp)
-// : repr a (fun p n -> wp (fun x -> p (Some (x, n))))
-// = fun n -> (f (), n)
-
-// sub_effect PURE ~> STEXN = lift_pure_stexn
+effect Exn (a:Type) (pre:Type0) (post:option a -> Type0) =
+  EXN a (fun p -> pre /\ (forall r. post r ==> p r))
 
 
-// effect StExn (a:Type) (pre:nat -> Type0) (post:nat -> option (a & nat) -> Type0) =
-//   STEXN a (fun p n -> pre n /\ (forall r. post n r ==> p r))
+
+type pre_t = nat -> Type0
+type post_t (a:Type) = option (a & nat) -> Type0
+type wp_t0 (a:Type) = post_t a -> pre_t
+
+unfold
+let monotonic_wp (#a:Type) (wp:wp_t0 a) : Type0 =
+  forall p q.
+    (forall r. p r ==> q r) ==>
+    (forall n. wp p n ==> wp q n)
+
+type wp_t (a:Type) =
+  wp:wp_t0 a{monotonic_wp wp}
+
+type repr (a:Type) (wp:wp_t a) =
+  n:nat -> EXN (a & nat) (fun p -> wp p n)
+
+inline_for_extraction
+let return (a:Type) (x:a)
+: repr a (fun p n -> p (Some (x, n)))
+= fun n -> (x, n)
+
+unfold
+let post_a (a:Type) (b:Type) (wp_g:a -> wp_t b) (p:post_t b) : post_t a =
+  fun r ->
+  match r with
+  | None -> p None
+  | Some r -> Prims.auto_squash (wp_g (Mktuple2?._1 r) p (Mktuple2?._2 r))
+
+let lemma_monotonic2 (#a:Type) (#b:Type) (wp_f:wp_t a) (wp_g:a -> wp_t b) (p:post_t b) (q:post_t b) (n:nat)
+: Lemma
+  (requires forall (r:option (a & nat)). post_a a b wp_g p r ==> post_a a b wp_g q r)
+  (ensures wp_f (post_a a b wp_g p) n ==> wp_f (post_a a b wp_g q) n)
+= let aux (p q:post_t a)
+    : Lemma ((forall r. p r ==> q r) ==> (forall n. wp_f p n ==> wp_f q n))
+    = () in
+  aux (post_a a b wp_g p) (post_a a b wp_g q)
+
+unfold
+let bind_wp0 (a:Type) (b:Type) (wp_f:wp_t a) (wp_g:a -> wp_t b) : post_t b -> pre_t =
+  fun p n -> wp_f (post_a a b wp_g p) n
+
+open FStar.Tactics
+
+unfold
+let bind_wp (a:Type) (b:Type) (wp_f:wp_t a) (wp_g:a -> wp_t b) : wp_t b
+= assert (monotonic_wp (bind_wp0 a b wp_f wp_g)) by
+    (norm [delta_only [`%monotonic_wp]];
+     let p_binder = forall_intro () in
+     let q_binder = forall_intro () in
+     ignore (implies_intro ());
+     ignore (forall_intro ());
+     norm [delta_only [`%bind_wp0]];
+     let wp_f_binder, wp_g_binder =
+       match (cur_binders ()) with
+       | _::_::wp_f::wp_g::_ -> wp_f, wp_g
+       | _ -> fail "" in
+     apply_lemma (`(lemma_monotonic2 (`#(binder_to_term wp_f_binder)) (`#(binder_to_term wp_g_binder)) (`#(binder_to_term p_binder)) (`#(binder_to_term q_binder))));
+     norm [delta_only [`%post_a]];
+     ignore (forall_intro ()));
+  bind_wp0 a b wp_f wp_g
+
+inline_for_extraction
+let bind (a:Type) (b:Type)
+  (wp_f:wp_t a) (wp_g:a -> wp_t b)
+  (f:repr a wp_f) (g:(x:a -> repr b (wp_g x)))
+: repr b (bind_wp a b wp_f wp_g)
+= fun n ->
+  let (x, n) = f n in
+  g x n
+
+inline_for_extraction
+let subcomp (a:Type)
+  (wp_f:wp_t a) (wp_g:wp_t a)
+  (f:repr a wp_f)
+: Pure (repr a wp_g)
+  (requires forall p n. wp_g p n ==> wp_f p n)
+  (ensures fun _ -> True)
+= f
+
+inline_for_extraction
+let if_then_else (a:Type)
+  (wp_f:wp_t a) (wp_g:wp_t a)
+  (f:repr a wp_f) (g:repr a wp_g)
+  (p:Type0)
+: Type
+= repr a
+  (fun post n ->
+    (p ==> wp_f post n) /\
+    ((~ p) ==> wp_g post n))
+
+reifiable reflectable
+layered_effect {
+  STEXN : a:Type -> wp:wp_t a -> Effect
+  with
+  repr = repr;
+  return = return;
+  bind = bind;
+  subcomp = subcomp;
+  if_then_else = if_then_else
+}
+
+inline_for_extraction
+let lift_pure_stexn (a:Type) (wp:pure_wp a{forall p q. (forall x. p x ==> q x) ==> (wp p ==> wp q)}) (f:unit -> PURE a wp)
+: repr a (fun p n -> wp (fun x -> p (Some (x, n))))
+= fun n -> (f (), n)
+
+sub_effect PURE ~> STEXN = lift_pure_stexn
 
 
-// (*** Application ***)
-
-// assume val get_n1
-// : n:nat ->
-//   Pure (option (nat * nat))
-//   (requires n > 0)
-//   (ensures fun r ->
-//     match r with
-//     | None -> True
-//     | Some (n1, n2) -> n1 == n /\ n2 == n + 1)
-
-// type flt = {
-//   n1 : nat;
-//   n2 : nat;
-//   n3 : i:nat{n1 > 0 /\ n2 = n1 + 1 /\ i = n2 + 1}
-// }
-
-// let get_flt (n:nat)
-// : Pure (option flt)
-//   (requires n > 0)
-//   (ensures fun r ->
-//     match r with
-//     | None -> True
-//     | Some flt -> flt.n1 == n)
-// = let r = get_n1 n in
-//   match r with
-//   | None -> None
-//   | Some (x, n) ->
-//     let r = get_n1 n in
-//     match r with
-//     | None -> None
-//     | Some (y, n) ->
-//       let r = get_n1 n in
-//       match r with
-//       | None -> None
-//       | Some (z, _) -> Some ({ n1 = x; n2 = y; n3 = z })
+effect StExn (a:Type) (pre:nat -> Type0) (post:nat -> option (a & nat) -> Type0) =
+  STEXN a (fun p n -> pre n /\ (forall r. post n r ==> p r))
 
 
-// inline_for_extraction
-// let get_n1_exn_ (n:nat)
-// : unit ->
-//   Pure (option (nat * nat))
-//   (requires n > 0)
-//   (ensures fun r ->
-//     match r with
-//     | None -> True
-//     | Some (n1, n2) -> n1 == n /\ n2 == n + 1)
-// = fun _ ->
-//   get_n1 n
+(*** Application ***)
 
-// inline_for_extraction
-// let get_n1_exn (n:nat)
-// : Exn (nat * nat)
-//   (requires n > 0)
-//   (ensures fun r ->
-//     match r with
-//     | None -> True
-//     | Some (n1, n2) -> n1 == n /\ n2 == n + 1)
-// = EXN?.reflect (get_n1_exn_ n)
+assume val get_n1
+: n:nat ->
+  Pure (option (nat * nat))
+  (requires n > 0)
+  (ensures fun r ->
+    match r with
+    | None -> True
+    | Some (n1, n2) -> n1 == n /\ n2 == n + 1)
 
-// inline_for_extraction
-// let get_flt_exn (n:nat)
-// : Exn flt
-//   (requires n > 0)
-//   (ensures fun r ->
-//     match r with
-//     | None -> True
-//     | Some flt -> flt.n1 == n)
-// = let x, n = get_n1_exn n in
-//   let y, n = get_n1_exn n in
-//   let z, _ = get_n1_exn n in
-//   { n1 = x; n2 = y; n3 = z}
+type flt = {
+  n1 : nat;
+  n2 : nat;
+  n3 : i:nat{n1 > 0 /\ n2 = n1 + 1 /\ i = n2 + 1}
+}
 
-// inline_for_extraction
-// let get_n1_stexn_ (_:unit)
-// : n:nat ->
-//   Exn (nat * nat)
-//   (requires n > 0)
-//   (ensures fun r ->
-//     match r with
-//     | None -> True
-//     | Some (n1, n2) -> n1 == n /\ n2 == n + 1)
-// = fun n -> get_n1_exn n
-
-// inline_for_extraction
-// let get_n1_stexn (_:unit)
-// : StExn nat
-//   (requires fun n -> n > 0)
-//   (ensures fun n r ->
-//     match r with
-//     | None -> True
-//     | Some (n1, n2) -> n1 == n /\ n2 == n + 1)
-// = STEXN?.reflect (get_n1_stexn_ ())
-
-// let get_n1_stexn2 (_:unit)
-// : StExn nat
-//   (requires fun n -> n > 0)
-//   (ensures fun _ _ -> True)
-// = let n = get_n1_stexn () in
-//   n
-
-// inline_for_extraction
-// let get_flt_stexn (_:unit)
-// : StExn flt
-//   (requires fun n -> n > 0)
-//   (ensures fun n r ->
-//     match r with
-//     | None -> True
-//     | Some (flt, _) -> flt.n1 == n)
-// = let x = get_n1_stexn () in
-//   let y = get_n1_stexn () in
-//   let z = get_n1_stexn () in
-//   { n1 = x; n2 = y; n3 = z}
+let get_flt (n:nat)
+: Pure (option flt)
+  (requires n > 0)
+  (ensures fun r ->
+    match r with
+    | None -> True
+    | Some flt -> flt.n1 == n)
+= let r = get_n1 n in
+  match r with
+  | None -> None
+  | Some (x, n) ->
+    let r = get_n1 n in
+    match r with
+    | None -> None
+    | Some (y, n) ->
+      let r = get_n1 n in
+      match r with
+      | None -> None
+      | Some (z, _) -> Some ({ n1 = x; n2 = y; n3 = z })
 
 
-// let get_flt_stexn_reified (n:nat)
-// : Pure (option (flt * nat))
-//   (requires n > 0)
-//   (ensures fun r ->
-//     match r with
-//     | None -> True
-//     | Some (flt, _) -> flt.n1 == n)
-// = reify (reify (get_flt_stexn ()) n) ()
+inline_for_extraction
+let get_n1_exn_ (n:nat)
+: unit ->
+  Pure (option (nat * nat))
+  (requires n > 0)
+  (ensures fun r ->
+    match r with
+    | None -> True
+    | Some (n1, n2) -> n1 == n /\ n2 == n + 1)
+= fun _ ->
+  get_n1 n
+
+inline_for_extraction
+let get_n1_exn (n:nat)
+: Exn (nat * nat)
+  (requires n > 0)
+  (ensures fun r ->
+    match r with
+    | None -> True
+    | Some (n1, n2) -> n1 == n /\ n2 == n + 1)
+= EXN?.reflect (get_n1_exn_ n)
+
+inline_for_extraction
+let get_flt_exn (n:nat)
+: Exn flt
+  (requires n > 0)
+  (ensures fun r ->
+    match r with
+    | None -> True
+    | Some flt -> flt.n1 == n)
+= let x, n = get_n1_exn n in
+  let y, n = get_n1_exn n in
+  let z, _ = get_n1_exn n in
+  { n1 = x; n2 = y; n3 = z}
+
+inline_for_extraction
+let get_n1_stexn_ (_:unit)
+: n:nat ->
+  Exn (nat * nat)
+  (requires n > 0)
+  (ensures fun r ->
+    match r with
+    | None -> True
+    | Some (n1, n2) -> n1 == n /\ n2 == n + 1)
+= fun n -> get_n1_exn n
+
+inline_for_extraction
+let get_n1_stexn (_:unit)
+: StExn nat
+  (requires fun n -> n > 0)
+  (ensures fun n r ->
+    match r with
+    | None -> True
+    | Some (n1, n2) -> n1 == n /\ n2 == n + 1)
+= STEXN?.reflect (get_n1_stexn_ ())
+
+let get_n1_stexn2 (_:unit)
+: StExn nat
+  (requires fun n -> n > 0)
+  (ensures fun _ _ -> True)
+= let n = get_n1_stexn () in
+  n
+
+inline_for_extraction
+let get_flt_stexn (_:unit)
+: StExn flt
+  (requires fun n -> n > 0)
+  (ensures fun n r ->
+    match r with
+    | None -> True
+    | Some (flt, _) -> flt.n1 == n)
+= let x = get_n1_stexn () in
+  let y = get_n1_stexn () in
+  let z = get_n1_stexn () in
+  { n1 = x; n2 = y; n3 = z}
+
+
+let get_flt_stexn_reified (n:nat)
+: Pure (option (flt * nat))
+  (requires n > 0)
+  (ensures fun r ->
+    match r with
+    | None -> True
+    | Some (flt, _) -> flt.n1 == n)
+= reify (reify (get_flt_stexn ()) n) ()
